src/HOL/IMP/Abs_Int_init.thy
@@ -1,6 +1,5 @@
 theory Abs_Int_init
-imports "~~/src/HOL/ex/Interpretation_with_Defs"
-        "~~/src/HOL/Library/While_Combinator"
+imports "~~/src/HOL/Library/While_Combinator"
         Vars Collecting Abs_Int_Tests
 begin
 
